Reinstate list_MEM_dec
It is required for the translation: list_MEM cannot be translated as is

CheckerScript.sml
@@ -1,5 +1,5 @@
 open preamble CheckerSpecTheory
- 
+
 val _ = new_theory "Checker";
 
 val EWIN_dec_def = Define `
@@ -32,18 +32,14 @@ val Valid_PileTally_dec2_def = Define `
 val _ = overload_on("list_MEM",``λl1 l2. set l1 ⊆ set l2``);
 val _ = overload_on("list_not_MEM",``λl1 l2. DISJOINT (set l1) (set l2)``);
 
-(*
 val list_MEM_dec_def = Define `
       (list_MEM_dec [] l ⇔ T)
    /\ (list_MEM_dec (h::t) l ⇔ (MEM h l) /\ (list_MEM_dec t l))`;
-*)
-(*
+
 val list_not_MEM_dec_def = Define `
         (list_not_MEM_dec  [] l ⇔ T)
      /\ (list_not_MEM_dec (h::t) l ⇔ (~ MEM h l) /\ (list_not_MEM_dec t l))`;
 
-*)
- 
 val less_than_quota_def = Define `
   less_than_quota qu l ls =
     EVERY (λh. get_cand_tally h l < qu) ls`;
@@ -59,7 +55,7 @@ val ELIM_CAND_dec_def = Define `
    (t = t') /\ (e = e')
    /\ (LENGTH (e ++ h) > st) /\ (LENGTH e < st)
    /\ (¬(NULL l)) /\ (ALL_DISTINCT l)
-   /\ (list_MEM (h++e) l)
+   /\ (list_MEM_dec (h++e) l)
    /\ (ALL_DISTINCT (h++e))
    /\ (Valid_PileTally_dec1 p l) /\ (Valid_PileTally_dec2 p l)
    /\ (Valid_PileTally_dec1 p' l) /\ (Valid_PileTally_dec2 p' l)
@@ -73,14 +69,14 @@ val ELIM_CAND_dec_def = Define `
    /\ (MEM (c,[]) p')
    /\ (subpile1 c p p') /\ (subpile2 c p' p) ) ∧
   (ELIM_CAND_dec _ _ _ _ = F)`;
- 
+
 val TRANSFER_dec_def = Define `
   (TRANSFER_dec ((qu,st,l):params)
     (NonFinal ([], t, p, bl, e, h))
     (NonFinal (ba', t', p', bl', e',h')) ⇔
       (e = e') /\ (h = h') /\ (t = t')
    /\ (LENGTH e < st)
-   /\ (list_MEM (h++e) l)
+   /\ (list_MEM_dec (h++e) l)
    /\ ALL_DISTINCT (h++e)
    /\ (Valid_PileTally_dec1 t l) /\ (Valid_PileTally_dec2 t l)
    /\ (Valid_PileTally_dec1 p l) /\ (Valid_PileTally_dec2 p l)
@@ -94,7 +90,7 @@ val TRANSFER_dec_def = Define `
          /\ (MEM (hbl,[]) p')
          /\ (subpile1 hbl p p') /\ (subpile2 hbl p' p))) ∧
   (TRANSFER_dec _ _ _ = F)`;
- 
+
 val first_continuing_cand_dec_def = Define `
   (first_continuing_cand_dec (c:cand) ([]: cand list)  (h: cand list) ⇔ F) /\
   (first_continuing_cand_dec c (b0::bs) h =
@@ -123,7 +119,7 @@ val COUNT_dec_def = Define `
     /\ (bl = bl') /\ (e = e') /\ (h = h')
     /\ ALL_DISTINCT (h++e)
     /\ ALL_DISTINCT (MAP FST p)
-    /\ (list_MEM (h++e) l)
+    /\ (list_MEM_dec (h++e) l)
     /\ (Valid_PileTally_dec1 t l) /\ (Valid_PileTally_dec2 t l)
     /\ (Valid_PileTally_dec1 t' l) /\ (Valid_PileTally_dec2 t' l)
     /\ (Valid_PileTally_dec1 p l) /\ (Valid_PileTally_dec2 p l)
@@ -136,21 +132,21 @@ val COUNT_dec_def = Define `
     /\ ~ (NULL h)
     /\ (ba' = [])) /\
    (COUNT_dec _ _ _ = F)`;
- 
- 
+
+
 val take_append_def = Define `
    (take_append (l0::ls) (h::t) = (take_append ls t)) ∧
    (take_append l1 _ = l1)`;
 
 val eqe_list_dec_def = Define `
-     (eqe_list_dec ([]: cand list) l1 l2 ⇔ list_MEM l1 l2)
+     (eqe_list_dec ([]: cand list) l1 l2 ⇔ list_MEM_dec l1 l2)
   /\ (eqe_list_dec (l0::ls) l1 l2 ⇔ (~ MEM l0 l1) /\ (MEM l0 l2) /\ eqe_list_dec ls l1 l2)`;
 
 
 val eqe_list_dec2_def = Define `
     eqe_list_dec2 l0 l1 l = EVERY (\l'. MEM l' l0 \/ MEM l' l1) l`
 
- 
+
 val bigger_than_quota = Define `
   bigger_than_quota ls (t:tallies) (qu:rat) =
     EVERY (λl0. qu ≤ get_cand_tally l0 t) ls`;
@@ -161,14 +157,14 @@ val piles_eq_list_def = Define `
           if ~ (MEM l0 l)
               then (get_cand_pile l0 p1 = get_cand_pile l0 p2) /\ (piles_eq_list ls l p1 p2)
           else (piles_eq_list ls l p1 p2))`;
- 
+
 val update_cand_pile = Define `
           (update_cand_pile (qu: rat) t ([]: cand list) p1 p2 ⇔ T)
        /\ (update_cand_pile qu t (l0::ls) p1 p2 ⇔
            (MAP FST (get_cand_pile l0 p2) = MAP FST (get_cand_pile l0 p1))
         /\ (MAP SND (get_cand_pile l0 p2) = update_cand_trans_val qu l0 t p1) /\
            update_cand_pile qu t ls p1 p2)`;
- 
+
 val ELECT_dec = Define `
      (ELECT_dec ((qu,st,l): params)
            (NonFinal (ba, t, p, bl, e, h))
@@ -200,11 +196,11 @@ val ELECT_dec = Define `
                 /\ (Valid_PileTally_dec1 p l) /\ (Valid_PileTally_dec2 p l)
                 /\ (Valid_PileTally_dec1 p' l) /\ (Valid_PileTally_dec2 p' l)
                 /\ (Valid_PileTally_dec1 t l) /\ (Valid_PileTally_dec2 t l)
-                /\ (list_MEM e' l)
-                /\ (list_MEM h l)
+                /\ (list_MEM_dec e' l)
+                /\ (list_MEM_dec h l)
                 /\ (update_cand_pile qu t l1 p p')) /\
      (ELECT_dec _ _ _ = F)`;
-  
+
 val Initial_Judgement_dec_def = Define `
         (Initial_Judgement_dec _ (Final _) ⇔ F)
      /\ (Initial_Judgement_dec l (NonFinal (ba, t, p, bl, e, h)) ⇔
@@ -213,7 +209,7 @@ val Initial_Judgement_dec_def = Define `
                              /\ (e = [])
                              /\ (h = l)
                              /\ (EVERY NULL (MAP SND p)))`;
- 
+
 val Valid_Step_def = Define`
   Valid_Step params j0 j1 ⇔
        HWIN_dec params j0 j1
@@ -230,7 +226,7 @@ val valid_judgements_dec_def = Define `
     /\ (valid_judgements_dec params (j0::j1::js) ⇔
         Valid_Step params j0 j1
         /\ (valid_judgements_dec params (j1::js)))`;
- 
+
 val valid_judgements_dec_ind = theorem"valid_judgements_dec_ind";
 
 val valid_judgments_dec_LRC = Q.store_thm("valid_judgments_dec_LRC",
